theories/iris/iris_atomicity.v
@@ -7,11 +7,9 @@ Require Export datatypes host operations properties opsem.
 
   (*
 Variable host_function : eqType.
-
 Let host := host.host host_function.
 Let function_closure := function_closure host_function.
 Let store_record := store_record host_function.
-
 Variable host_instance : host.
 *)
 
@@ -28,6 +26,8 @@ Definition is_atomic (e : expr) : Prop :=
   match e with
   | [::AI_basic (BI_const (VAL_int32 _)); AI_basic (BI_load _ _ _ _)] => True
   | [::AI_basic (BI_const (VAL_int32 _)); AI_basic (BI_const _); AI_basic (BI_store _ _ _ _)] => True
+  | [::AI_basic (BI_const _); AI_basic (BI_set_global _)] => True
+  | [::AI_basic (BI_get_global _)] => True
   | [::AI_trap] => True
   | _ => False
   end.
@@ -41,17 +41,20 @@ Lemma is_atomic_eq (e : expr) :
   is_atomic e ->
   (∃ k x1 x2 x3 x4, e = [::AI_basic (BI_const (VAL_int32 k)); AI_basic (BI_load x1 x2 x3 x4)]) ∨
   (∃ k v x1 x2 x3 x4, e = [::AI_basic (BI_const (VAL_int32 k)); AI_basic (BI_const v); AI_basic (BI_store x1 x2 x3 x4)]) ∨
+  (∃ v g, e = [::AI_basic (BI_const v); AI_basic (BI_set_global g)]) ∨
+  (∃ g, e = [::AI_basic (BI_get_global g)]) ∨
   (e = [::AI_trap]).
 Proof.
   intros He.
   do 2 (destruct e;try done).
   { destruct a;try done.
-    destruct b;try done; destruct v;try done.
-    right. by right. }
+    destruct b;try done. right. right. right. left. eauto.
+    destruct v;try done.
+    right. right. right. by right. }
   do 1 (destruct e;try done).
   { revert He. cbn. repeat destruct_match_goal.
-    move => *.
-    left. repeat eexists. } 
+    all: try by (move => *; right; right; left; repeat eexists).
+    move => *. left. repeat eexists. } 
   { destruct e.
     2: { exfalso. cbn in He. revert He.
          repeat destruct_match_goal. }
@@ -110,7 +113,47 @@ Proof.
   pose proof (reduce_not_nil Hred) as Hnil.
   destruct vs,es,es'0 => //=.
   all: do 2 (try destruct vs; try destruct es; try destruct es'0 => //=;simplify_eq).
-Qed.  
+Qed.
+
+Lemma reduce_set_global_false s0 f s' f' es es' g :
+  es = [AI_basic (BI_set_global g)] ->
+  reduce s0 f es s' f' es' -> False.
+Proof.
+  intros Heq Hred.
+  apply Logic.eq_sym in Heq.
+  no_reduce Heq Hred.
+Qed.
+
+Lemma atomic_no_hole_set_global s0 f es s' f' es' k lh v g :
+  reduce s0 f es s' f' es' ->
+  lfilled k lh es [::AI_basic (BI_const v); AI_basic (BI_set_global g)] ->
+  lh = LH_base [] [] ∧ k = 0.
+Proof.
+  intros Hred Hfill.
+  apply lfilled_Ind_Equivalent in Hfill.
+  destruct k;inversion Hfill;subst;[split;auto|repeat destruct vs => //=].
+  pose proof (reduce_not_nil Hred) as Hnil.
+  destruct vs,es,es'0 => //=.
+  all: do 3 (try destruct vs; try destruct es; try destruct es'0 => //=;simplify_eq).
+  { inversion H;subst. exfalso.
+    eapply reduce_val_false;eauto. eauto. }
+  { inversion H;subst. exfalso.
+    eapply reduce_set_global_false;eauto. }
+Qed.
+
+Lemma atomic_no_hole_get_global s0 f es s' f' es' k lh g:
+  reduce s0 f es s' f' es' -> 
+  lfilled k lh es [::AI_basic (BI_get_global g)] ->
+  lh = LH_base [] [] ∧ k = 0.
+Proof.
+  intros Hred Hfill.
+  apply lfilled_Ind_Equivalent in Hfill.
+  destruct k;inversion Hfill;subst;[split;auto|repeat destruct vs => //=].
+  pose proof (reduce_not_nil Hred) as Hnil.
+  destruct vs,es,es'0 => //=.
+  all: do 2 (try destruct vs; try destruct es; try destruct es'0 => //=;simplify_eq).
+Qed.
+  
 
 Global Instance is_atomic_correct s e : is_atomic e → @Atomic wasm_lang s e.
 Proof.
@@ -122,11 +165,15 @@ Proof.
   destruct Hstep as [Hstep [-> ->]].
   induction Hstep using reduce_ind.
   all: apply is_atomic_eq in Ha as Heq.
-  all: destruct Heq as [(?&?&?&?&?&?)|[(?&?&?&?&?&?&?)|?]];simplify_eq; eauto.
+  all: destruct Heq as [(?&?&?&?&?&?)|[(?&?&?&?&?&?&?)|[(?&?&?)|[(?&?)|?]]]];simplify_eq; eauto.
   all: try by (do 2 (destruct vcs;try done)).
   all: try by (do 3 (destruct vcs;try done)).
   { inversion H;subst;eauto.
     1,2: do 3 (destruct vs;try done). }
+  { inversion H;subst;eauto.
+    1,2: do 4 (destruct vs;try done). }
+  { inversion H;subst;eauto.
+    1,2: do 4 (destruct vs;try done). }
   { inversion H;subst;eauto.
     1,2: do 4 (destruct vs;try done). }
   { inversion H;simpl;eauto; subst; exfalso.
@@ -143,6 +190,18 @@ Proof.
     apply lfilled_Ind_Equivalent in H0.
     inversion H;inversion H0; subst. erewrite app_nil_r in H3. subst.
     erewrite app_nil_r. erewrite app_nil_l. apply IHHstep. auto. }
+  { edestruct atomic_no_hole_set_global as [Hlh Hk];eauto.
+    subst k. subst lh.
+    apply lfilled_Ind_Equivalent in H.
+    apply lfilled_Ind_Equivalent in H0.
+    inversion H;inversion H0; subst. erewrite app_nil_r in H3. subst.
+    erewrite app_nil_r. erewrite app_nil_l. apply IHHstep. auto. }
+  { edestruct atomic_no_hole_get_global as [Hlh Hk];eauto.
+    subst k. subst lh.
+    apply lfilled_Ind_Equivalent in H.
+    apply lfilled_Ind_Equivalent in H0.
+    inversion H;inversion H0; subst. erewrite app_nil_r in H3. subst.
+    erewrite app_nil_r. erewrite app_nil_l. apply IHHstep. auto. }  
   { edestruct atomic_no_hole_trap as [Hlh Hk];eauto.
     subst k. subst lh.
     apply lfilled_Ind_Equivalent in H.
